Splinter/AllocationTable.i.dfy
@@ -1,0 +1,16 @@
+// Copyright 2018-2021 VMware, Inc., Microsoft Inc., Carnegie Mellon University, ETH Zurich, and University of Washington
+// SPDX-License-Identifier: BSD-2-Clause
+
+include "../lib/Base/Option.s.dfy"
+include "Allocation.i.dfy"
+include "CacheIfc.i.dfy"
+include "MarshalledSnapshot.i.dfy"
+
+module AllocationTableMod {
+  import opened Options
+  import opened AllocationTableMachineMod
+
+  function I(dv: AllocationMod.DiskView, sb: Superblock) : Option<AllocationTable> {
+    parse(IBytes(dv, sb.snapshot))
+  }
+}
