Splinter/BetreeInterp.i.dfy
@@ -2,7 +2,9 @@
 // SPDX-License-Identifier: BSD-2-Clause
 
 include "../lib/Base/total_order.i.dfy"
-include "Tables.i.dfy"
+include "IndirectionTable.i.dfy"
+include "AllocationTable.i.dfy"
+include "AllocationTableMachine.i.dfy"
 include "MsgSeq.i.dfy"
 include "Betree.i.dfy"
 include "Message.s.dfy"
