Splinter/IndirectionTable.i.dfy
@@ -1,0 +1,33 @@
+// Copyright 2018-2021 VMware, Inc., Microsoft Inc., Carnegie Mellon University, ETH Zurich, and University of Washington
+// SPDX-License-Identifier: BSD-2-Clause
+
+include "../lib/Base/Option.s.dfy"
+include "Allocation.i.dfy"
+include "CacheIfc.i.dfy"
+include "MarshalledSnapshot.i.dfy"
+
+module IndirectionTableMod refines MarshalledSnapshot {
+  import CacheIfc
+
+  datatype Superblock = Superblock(snapshot: SnapshotSuperblock)
+
+  function EmptySuperblock() : Superblock
+  {
+    Superblock(SnapshotSuperblock(None))
+  }
+
+  type IndirectionTable = map<nat, CU>
+
+  function parse(b: seq<byte>) : Option<IndirectionTable>
+
+  function I(dv: DiskView, sb: Superblock) : Option<IndirectionTable> {
+    parse(IBytes(dv, sb.snapshot))
+  }
+
+  predicate DurableAt(itbl: IndirectionTable, cache: CacheIfc.Variables, sb: Superblock)
+  {
+    // TODO kind of dirty peeking into the entire cache here
+    // ValidSnapshot(cache.dv, sb.snapshot)
+    true
+  }
+}
