Splinter/ProofObligations.s.dfy
@@ -1,0 +1,33 @@
+// Copyright 2018-2021 VMware, Inc., Microsoft Inc., Carnegie Mellon University, ETH Zurich, and University of Washington
+// SPDX-License-Identifier: BSD-2-Clause
+
+include "Spec.s.dfy"
+include "../lib/Base/MapRemove.s.dfy"
+include "../lib/Checksums/CRC32C.s.dfy"
+include "AsyncDisk.s.dfy"
+include "AsyncDiskProgram.s.dfy"
+
+abstract module ProofObligations {
+  import CrashTolerantMapSpecMod
+  import ConcreteSystem : IOSystem
+
+  // Your interpretation function
+  function I(v: ConcreteSystem.Variables) : CrashTolerantMapSpecMod.Variables
+
+  // Your system invariant
+  predicate Inv(v: ConcreteSystem.Variables)
+
+  lemma InitRefines(v: ConcreteSystem.Variables)
+    requires ConcreteSystem.Init(v)
+    ensures CrashTolerantMapSpecMod.Init(I(v))
+
+  lemma InvInductive(v: ConcreteSystem.Variables, v': ConcreteSystem.Variables, uiop: ConcreteSystem.UIOp)
+    requires Inv(v)
+    requires ConcreteSystem.Next(v, v', uiop)
+    ensures Inv(v')
+
+  lemma NextRefines(v: ConcreteSystem.Variables, v': ConcreteSystem.Variables, uiop: ConcreteSystem.UIOp)
+    requires Inv(v)
+    requires ConcreteSystem.Next(v, v', uiop)
+    ensures CrashTolerantMapSpecMod.Next(I(v), I(v'), uiop)
+}
